Upgrade stdpp 1.8.0 and Iris 4.0.0

theories/finz_base.v
@@ -16,7 +16,7 @@ Definition to_z (f: finz): Z :=
 
 Definition of_z (z : Z) : option finz.
 Proof.
-  destruct (Z_lt_dec z finz_bound),(Z_le_dec 0%Z z).
+  destruct (Z.lt_dec z finz_bound),(Z.le_dec 0%Z z).
   - apply (Z.ltb_lt z finz_bound) in l.
     apply (Z.leb_le 0 z) in l0.
     exact (Some (FinZ z l l0)).
@@ -40,9 +40,9 @@ Definition eqb : finz → finz → bool :=
 
 Program Definition incr (f : finz) (off : Z) : option finz :=
   let z := (to_z f + off)%Z in
-  match (Z_lt_dec z finz_bound) with
+  match (Z.lt_dec z finz_bound) with
   | left _ =>
-    match (Z_le_dec 0%Z z) with
+    match (Z.le_dec 0%Z z) with
     | left _ => Some (FinZ z _ _)
     | right _ => None
     end
@@ -79,9 +79,9 @@ Definition incr_default (f : finz) (off : Z) : finz :=
 
 Program Definition mult (f : finz) (off : Z) : option finz :=
   let z := (to_z f * off)%Z in
-  match (Z_lt_dec z finz_bound) with
+  match (Z.lt_dec z finz_bound) with
   | left _ =>
-    match (Z_le_dec 0%Z z) with
+    match (Z.le_dec 0%Z z) with
     | left _ => Some (FinZ z _ _)
     | right _ => None
     end
@@ -174,7 +174,7 @@ Qed.
 
 Global Instance finz_eq_dec : EqDecision (finz finz_bound).
 Proof.
-  intros x y. destruct x as [x],y as [y]. destruct (Z_eq_dec x y).
+  intros x y. destruct x as [x],y as [y]. destruct (Z.eq_dec x y).
   - left. eapply finz_to_z_eq; eauto.
   - right. inversion 1. simplify_eq.
 Defined.
@@ -192,8 +192,8 @@ Proof.
   generalize (finz_spec f); intros [? ?].
   set (z := (finz.to_z f)) in *.
   unfold finz.of_z.
-  destruct (Z_lt_dec z finz_bound) eqn:?;
-  destruct (Z_le_dec 0%Z z) eqn:?.
+  destruct (Z.lt_dec z finz_bound) eqn:?;
+  destruct (Z.le_dec 0%Z z) eqn:?.
   { f_equal. apply finz_to_z_eq. cbn. lia. }
   all: lia.
 Qed.
@@ -225,7 +225,7 @@ Proof.
   intro r. destruct r; auto.
   rewrite decode_encode.
   unfold finz.of_z. simpl.
-  destruct (Z_lt_dec z finz_bound),(Z_le_dec 0%Z z).
+  destruct (Z.lt_dec z finz_bound),(Z.le_dec 0%Z z).
   - repeat f_equal; apply eq_proofs_unicity; decide equality.
   - exfalso. by apply (Z.leb_le 0 z) in finz_nonneg.
   - exfalso. by apply (Z.ltb_lt z finz_bound) in finz_lt.
@@ -236,13 +236,13 @@ Defined.
 Global Instance finz_le_dec : RelDecision (@finz.le finz_bound).
 Proof.
   intros x y. destruct x as [x], y as [y].
-  destruct (Z_le_dec x y); [by left|by right].
+  destruct (Z.le_dec x y); [by left|by right].
 Defined.
 
 Global Instance finz_lt_dec : RelDecision (@finz.lt finz_bound).
 Proof.
   intros x y. destruct x as [x], y as [y].
-  destruct (Z_lt_dec x y); [by left|by right].
+  destruct (Z.lt_dec x y); [by left|by right].
 Defined.
 
 Global Instance finz_le_trans : Transitive (@finz.le finz_bound).
